finish chapter04

exercises/chapter04-invariants/exercise01.dfy
@@ -33,7 +33,7 @@ module Crawler {
 
   ghost predicate Inv(v:Variables) {
     // FIXME: fill in here (solution: 1 line)
-     true  // probably not strong enough. :v)
+    v.x + v.y >= 5
     // END EDIT
   }
 
